src/mTranslate.mli
@@ -1,8 +1,0 @@
-open Globnames
-
-val string_of_chars : char list -> string
-val chars_of_string : string -> char list
-
-val translate : Environ.env -> Typing0.global_context -> Trad.tsl_context -> Evd.evar_map -> Constr.t -> Constr.t * Evd.evar_map
-
-val translate_type : Environ.env -> Typing0.global_context -> Trad.tsl_context -> Evd.evar_map -> Constr.t -> Constr.t * Evd.evar_map
