src/unquote.mli
@@ -1,0 +1,6 @@
+open Globnames
+
+val string_of_chars : char list -> string
+val chars_of_string : string -> char list
+
+val unquote : Evd.evar_map -> Ast0.term -> Evd.evar_map * Term.constr
