theories/translation_utils.v
@@ -1,0 +1,74 @@
+Require Import Template.Ast Template.Typing Template.Checker.
+Require Import List.
+Import ListNotations.
+
+
+Definition tsl_context := list (ident * ident).
+
+Fixpoint lookup_tsl_ctx (E : tsl_context) (id : ident) : option ident :=
+  match E with
+  | nil => None
+  | hd :: tl =>
+    if ident_eq id (fst hd) then Some (snd hd)
+    else lookup_tsl_ctx tl id
+  end.
+
+
+Section MonadMap.
+  Import MonadNotation.
+  Context {T} {M : Monad T}.
+
+  Fixpoint monad_map {A} {B} (f : A -> T B) (l : list A) : T (list B)
+    := match l with
+       | nil => ret nil
+       | x :: l => x' <- f x ;;
+                  l' <- monad_map f l ;;
+                  ret (x' :: l')
+       end.
+End MonadMap.
+
+
+Inductive tsl_error :=
+| NotEnoughFuel : tsl_error
+| TranslationNotFound : ident -> tsl_error
+| TranslationNotHandeled
+| TypingError.
+
+Inductive tsl_result A :=
+| Success : A -> tsl_result A
+| Error : tsl_error -> tsl_result A.
+
+Instance tsl_monad : Monad tsl_result :=
+  {| ret A a := Success A a ;
+     bind A B m f :=
+       match m with
+       | Success _ a => f a
+       | Error _ e => Error _ e
+       end
+  |}.
+
+Instance monad_exc : MonadExc tsl_error tsl_result :=
+  { raise A e := Error A e;
+    catch A m f :=
+      match m with
+      | Success _ a => m
+      | Error _ t => f t
+      end
+  }.
+
+
+Require Import Template.Template Template.sigma.
+
+Quote Definition tSigma := sigma.
+Quote Definition tPair := @mk_sig.
+Definition pair (typ1 typ2 t1 t2 : term) : term
+  := tApp tPair [ typ1 ; typ2 ; t1 ; t2].
+Definition pack (t u : term) : term
+  := tApp tSigma [ t ; u ].
+Definition proj1 (t : term) : term
+  := tProj (mkInd "Template.sigma.sigma" 0, 2, 0) t.
+Definition proj2 (t : term) : term
+  := tProj (mkInd "Template.sigma.sigma" 0, 2, 1) t.
+Definition proj (b : bool) (t : term) : term
+  := tProj (mkInd "Template.sigma.sigma" 0, 2, if b then 0 else 1) t.
+
